Registers.thy
@@ -4,21 +4,14 @@ begin
 
 section "Simps"
 
-lemma memory_\<alpha>_eq[simp]: "memory_\<alpha> (l,g,s,h) = memory_\<alpha> (l',g',s,h)"
+lemma memory_\<alpha>_eq[simp]: "memory_\<alpha> (lr,gr,sm,hm,gm) = memory_\<alpha> (lr',gr',sm,hm,gm)"
   apply (rule ext)
   subgoal for x
     by (cases x; simp)
   done
 
 lemma register_\<alpha>_lid_update_eq[simp]:
-  "register_\<alpha> (Mapping.update n v l, g, s, h) = (register_\<alpha> (l, g, s, h))(reg (lid n) := Some v)"
-  apply (auto simp: fun_eq_iff split: llvm_value_ref.split)
-  subgoal for x apply (cases x; simp) subgoal for id by (cases id; simp)
-  done
-  done
-
-lemma register_\<alpha>_gid_update_eq[simp]:
-  "register_\<alpha> (l, Mapping.update n v g, s, h) = (register_\<alpha> (l, g, s, h))(reg (gid n) := Some v)"
+  "register_\<alpha> (Mapping.update n v lr,gr,sm,hm,gm) = (register_\<alpha> (lr,gr,sm,hm,gm))(reg (lid n) := Some v)"
   apply (auto simp: fun_eq_iff split: llvm_value_ref.split)
   subgoal for x apply (cases x; simp) subgoal for id by (cases id; simp)
   done
@@ -33,17 +26,17 @@ lemma register_\<alpha>_update_independent[simp]:
   by (metis fun_upd_other)
 
 lemma register_\<alpha>_eq_get_register:
-  "register_\<alpha> s v = Some v' \<longleftrightarrow> get_register s v = ok v'"
+  "register_\<alpha> s v = Some v' \<longleftrightarrow> dereference s v = ok v'"
   apply (cases s; cases v; auto)
-  subgoal for _ _ _ _ n by (cases n; simp)
-  subgoal for _ _ _ _ n by (cases n; simp split: option.splits)
+  subgoal for _ _ _ _ _ n by (cases n; simp split: option.splits)
+  subgoal for _ _ _ _ _ n by (cases n; simp split: option.splits)
   done
 
 
 section "register_\<alpha> operation"
 
 lemma set_register_\<alpha>:
-  "register_\<alpha> (set_register n v s) = (register_\<alpha> s)(reg n := Some v)"
+  "set_register n v s = ok s' \<Longrightarrow> register_\<alpha> s' = (register_\<alpha> s)(reg n := Some v)"
   apply (cases s; rule ext)
   subgoal for l' g' s' h' x by (cases x; cases n; auto simp: set_single_register_def)
   done
@@ -55,25 +48,22 @@ section "Intro rules"
 named_theorems register_intro
 
 lemma wp_set_single_register_lid_intro[THEN consequence, register_intro]:
-  "wp (return (set_single_register n v l,g,s,h)) (\<lambda>s'. register_\<alpha> s' = (register_\<alpha> (l,g,s,h))(reg (lid n) := Some v) \<and> memory_\<alpha> s' = memory_\<alpha> (l,g,s,h))"
-  unfolding set_single_register_def
-  by (intro wp_intro wp_return_intro; simp)
-
-lemma wp_set_single_register_gid_intro[THEN consequence, register_intro]:
-  "wp (return (l,set_single_register n v g,s,h)) (\<lambda>s'. register_\<alpha> s' = (register_\<alpha> (l,g,s,h))(reg (gid n) := Some v) \<and> memory_\<alpha> s' = memory_\<alpha> (l,g,s,h))"
+  "wp (return (set_single_register n v lr,gr,sm,hm,gm)) (\<lambda>s'. register_\<alpha> s' = (register_\<alpha> (lr,gr,sm,hm,gm))(reg (lid n) := Some v) \<and> memory_\<alpha> s' = memory_\<alpha> (lr,gr,sm,hm,gm))"
   unfolding set_single_register_def
   by (intro wp_intro wp_return_intro; simp)
 
 lemma wp_set_register_intro[THEN consequence, wp_intro]:
-  shows "wp (return (set_register n v s)) (\<lambda>s'. register_\<alpha> s' = (register_\<alpha> s)(reg n := Some v) \<and> memory_\<alpha> s' = memory_\<alpha> s)"
-  by (cases n; cases s; simp; intro wp_intro register_intro; simp)
+  assumes "is_lid n"
+  shows "wp (set_register n v s) (\<lambda>s'. register_\<alpha> s' = (register_\<alpha> s)(reg n := Some v) \<and> memory_\<alpha> s' = memory_\<alpha> s)"
+  using assms
+  by (cases n; cases s; simp; intro wp_intro register_intro; simp add: set_single_register_def)
 
 
 lemma wp_get_register_intro[THEN consequence, wp_intro]:        
   assumes "register_\<alpha> s n \<noteq> None"
-  shows "wp (get_register s n) (\<lambda>v'. register_\<alpha> s n = Some v')"
+  shows "wp (dereference s n) (\<lambda>v'. register_\<alpha> s n = Some v')"
   using assms
-  apply (cases s; cases n) subgoal for _ _ _ _ id by (cases id; simp; intro wp_intro; auto)
+  apply (cases s; cases n) subgoal for _ _ _ _ _ id by (cases id; simp; intro wp_intro; auto split: option.splits)
   by simp
 
 
